matching-logic/src/Theories/Definedness.v
@@ -3306,6 +3306,144 @@ Proof.
   apply Singleton_ctx. exact wfϕ.
 Defined.
 
+Lemma membership_symbol_ceil_right {Σ : Signature} {syntax : Syntax} Γ ϕ x:
+  theory ⊆ Γ ->
+  well_formed ϕ ->
+  Γ ⊢ ((ex, (BoundVarSugar.b0 ∈ml ϕ)) ---> (patt_free_evar x ∈ml ⌈ ϕ ⌉)).
+Proof.
+  intros HΓ wfϕ.
+  remember (evar_fresh (elements ({[x]} ∪ (free_evars ϕ)))) as y.
+  pose proof (Htmp := @set_evar_fresh_is_fresh' Σ ({[x]} ∪ free_evars ϕ)).
+  rewrite -Heqy in Htmp.
+  assert (x <> y).
+  { solve_fresh_neq. }
+
+  eapply syllogism_intro.
+  1,3: wf_auto2.
+  2: {
+    apply (@strip_exists_quantify_l Σ Γ y).
+    { simpl. clear -Htmp. set_solver. }
+    { simpl. split_and!; try reflexivity. wf_auto2. }
+    apply ex_quan_monotone.
+    { wf_auto2. }
+    2: {
+      unfold evar_open. simpl_bevar_subst. simpl.
+      rewrite bevar_subst_not_occur.
+      { apply wfc_ex_aux_implies_not_bevar_occur. wf_auto2. }
+      apply membership_symbol_ceil_aux_0 with (y0 := x); assumption.
+    }
+    { wf_auto2. }
+  }
+  { unfold exists_quantify. simpl. repeat case_match; try congruence; wf_auto2. }
+
+  eapply syllogism_intro.
+  3: wf_auto2.
+  1: { unfold exists_quantify. simpl. repeat case_match; try congruence; wf_auto2. }
+  2: {
+    apply pf_iff_proj2.
+    2: { unfold exists_quantify. simpl. repeat case_match; try congruence; wf_auto2. }
+    2: { 
+      unfold exists_quantify. simpl.
+      repeat case_match; try congruence; try contradiction.
+      apply membership_exists.
+      { exact HΓ. }
+      { wf_auto2. }
+    }
+    { wf_auto2. }
+  }
+  { wf_auto2. }
+
+  eapply syllogism_intro.
+  1,3: wf_auto2.
+  2: {
+    apply membership_monotone.
+    { exact HΓ. }
+    { wf_auto2. }
+    2: {
+    apply (@strip_exists_quantify_l Σ Γ y).
+    { simpl.
+      rewrite evar_quantify_free_evar_subst.
+      { apply count_evar_occurrences_0.
+        subst y.
+        eapply evar_is_fresh_in_richer'.
+        2: { apply set_evar_fresh_is_fresh'. }
+        clear. set_solver.
+      }
+      set_solver.
+    }
+    { simpl. split_and!; try reflexivity. wf_auto2. }
+    apply ex_quan_monotone.
+    { wf_auto2. }
+    2: {
+      eapply syllogism_intro.
+      1: wf_auto2.
+      3: {
+        unfold evar_open. simpl_bevar_subst. simpl.
+        rewrite bevar_subst_evar_quantify_free_evar.
+        { apply wfc_ex_implies_not_bevar_occur. wf_auto2. }
+        apply membership_symbol_ceil_aux_0 with (y0 := y); assumption.
+      }
+      { wf_auto2. }
+      2: {
+        apply ceil_monotonic.
+        { exact HΓ. }
+        { wf_auto2. }
+        2: {
+          eapply pf_iff_proj1.
+          { wf_auto2. }
+          2: {
+            apply patt_and_comm.
+            { wf_auto2. }
+            { wf_auto2. }
+          }
+          { wf_auto2. }
+        }
+        { wf_auto2. }
+      }
+      { wf_auto2. }
+    }
+    { wf_auto2. }
+  }
+  { unfold exists_quantify. simpl. repeat case_match; try congruence; wf_auto2. }
+  }
+  { unfold exists_quantify. simpl. repeat case_match; try congruence; wf_auto2. }
+
+  eapply syllogism_intro.
+  { unfold exists_quantify. simpl. repeat case_match; try congruence; wf_auto2. }
+  2: { wf_auto2. }
+  2: {
+    apply membership_monotone.
+    { exact HΓ. }
+    { unfold exists_quantify. simpl. repeat case_match; try congruence; wf_auto2. } 
+    2: {
+      unfold exists_quantify.
+      simpl.
+      repeat case_match; try congruence.
+      rewrite evar_quantify_free_evar_subst.
+      { apply count_evar_occurrences_0.
+        subst y.
+        eapply evar_is_fresh_in_richer'.
+        2: { apply set_evar_fresh_is_fresh'. }
+        clear. set_solver.
+      }
+      apply ceil_propagation_exists_2.
+      { exact HΓ. }
+      { wf_auto2. }
+    }
+    { wf_auto2. }
+  }
+  { wf_auto2. }
+  apply membership_monotone.
+  { exact HΓ. }
+  { wf_auto2. }
+  { wf_auto2. }
+  apply ceil_monotonic.
+  { exact HΓ. }
+  { wf_auto2. }
+  { wf_auto2. }  
+  apply membership_symbol_ceil_right_aux_0; assumption.
+Defined.
+
 Lemma def_phi_impl_tot_def_phi {Σ : Signature} {syntax : Syntax} Γ ϕ :
   theory ⊆ Γ ->
   well_formed ϕ ->
@@ -3382,13 +3520,12 @@ Proof.
     reflexivity.
   }
 
-
-  assert (Htmp: Γ ⊢ (! (ex, b0 ∈ml ⌈ ϕ ⌉)) ---> (! (patt_free_evar x ∈ml ⌈ ϕ ⌉))).
+  assert (Htmp: Γ ⊢ (! (ex, b0 ∈ml ϕ)) ---> (! (patt_free_evar x ∈ml ⌈ ϕ ⌉))).
   {
     apply ProofMode.modus_tollens.
     { wf_auto2. }
     { wf_auto2. }
-    admit.
+    apply membership_symbol_ceil_left; assumption.
   }
   mgApplyMeta Htmp.
   fromMyGoal. intros _ _.
@@ -3423,12 +3560,30 @@ Proof.
     set_solver.
   }
 
-  Search patt_in "sym".
-  Search ML_proof_system patt_forall.
-  (* HERE *)
-  (* lemma-ceil-imp-floor-ceil *)
-Abort.
+  rewrite evar_quantify_evar_open.
+  { simpl. unfold evar_is_fresh_in in Hfr'. subst x. set_solver. }
+  unfold evar_open. simpl_bevar_subst. simpl.
+  rewrite bevar_subst_not_occur.
+  { apply wfc_ex_aux_implies_not_bevar_occur. wf_auto2. }
+  apply  membership_symbol_ceil_right; assumption.
+Defined.
 
+Lemma def_tot_phi_impl_tot_phi {Σ : Signature} {syntax : Syntax} Γ ϕ :
+  theory ⊆ Γ ->
+  well_formed ϕ ->
+  Γ ⊢ ⌈ ⌊ ϕ ⌋ ⌉ ---> ⌊ ϕ ⌋ .
+Proof.
+  intros HΓ wfϕ.
+  toMyGoal.
+  { wf_auto2. }
+  mgIntro.
+  mgApplyMeta (@not_not_intro Σ Γ (⌈ ⌊ ϕ ⌋ ⌉) ltac:(wf_auto2)) in 0.
+  mgIntro. mgApply 0. mgClear 0.
+  fromMyGoal. intros _ _.
+  apply def_phi_impl_tot_def_phi.
+  { exact HΓ. }
+  { wf_auto2. }
+Defined.
 
 Lemma floor_is_predicate {Σ : Signature} {syntax : Syntax} Γ ϕ :
   theory ⊆ Γ ->
@@ -3466,8 +3621,16 @@ Proof.
   toMyGoal.
   { wf_auto2. }
   mgRewrite H at 1.
-  (* TODO ceil-floor-imp-floor , ceil-imp-floor-ceil*)
-Abort.
+  clear H.
+  mgIntro.
+  mgApplyMeta (@def_phi_impl_tot_def_phi Σ syntax Γ (⌊ ϕ ⌋) HΓ ltac:(wf_auto2)) in 0.
+  fromMyGoal. intros _ _.
+  apply floor_monotonic.
+  { exact HΓ. }
+  { wf_auto2. }
+  { wf_auto2. }
+  apply def_tot_phi_impl_tot_phi; assumption.
+Defined.
 
 Lemma def_def_phi_impl_tot_def_phi {Σ : Signature} {syntax : Syntax} Γ ϕ :
   theory ⊆ Γ ->
